experiments/CSR.v
@@ -15,8 +15,8 @@ Import sv.
 Section csr.
 
 Notation "'mval'" := ("m_val":var) (in custom trm at level 0) : trm_scope.
-Notation "'colind'" := ("col_ind":var) (in custom trm at level 0) : trm_scope.
-Notation "'rowptr'" := ("row_ptr":var) (in custom trm at level 0) : trm_scope.
+Notation "'mind'" := ("m_ind":var) (in custom trm at level 0) : trm_scope.
+Notation "'mcrd'" := ("m_crd":var) (in custom trm at level 0) : trm_scope.
 Notation "'dvec'" := ("d_vec":var) (in custom trm at level 0) : trm_scope.
 Notation "'lb'" := ("l_b":var) (in custom trm at level 0) : trm_scope.
 Notation "'rb'" := ("r_b":var) (in custom trm at level 0) : trm_scope.
@@ -24,56 +24,60 @@ Notation "'i''" := ("i_'":var) (in custom trm at level 0) : trm_scope.
 
 Import List Vars list_interval_notation.
 
-Context (mval colind rowptr : list int).
+Context (mval mind mcrd : list int).
 Context (N Nrow Ncol : int).
 Hypothesis Nrow_nonneg : 0 <= Nrow.
 Hypothesis len_mval : length mval = N :> int.
-Hypothesis len_colind : length colind = N :> int.
-Hypothesis len_rowptr : length rowptr = Nrow + 1 :> int.
-Hypothesis colind_leq : forall x, In x colind -> 0 <= x < Ncol.
-Hypothesis rowptr_first : List.nth (abs 0) rowptr 0 = 0.
-Hypothesis rowptr_last : List.nth (abs Nrow) rowptr 0 = N.
-Hypothesis rowptr_weakly_sorted : forall (i j : int), 
+Hypothesis len_mind : length mind = N :> int.
+Hypothesis len_mcrd : length mcrd = Nrow + 1 :> int.
+Hypothesis mind_leq : forall x, In x mind -> 0 <= x < Ncol.
+Hypothesis mcrd_first : List.nth (abs 0) mcrd 0 = 0.
+Hypothesis mcrd_last : List.nth (abs Nrow) mcrd 0 = N.
+Hypothesis mcrd_weakly_sorted : forall (i j : int), 
   (0 <= i <= Nrow) -> 
   (0 <= j <= Nrow) -> 
   (i <= j) -> 
-  (rowptr[i] <= rowptr[j]).
+  (mcrd[i] <= mcrd[j]).
 
-Definition colind_seg (row : int) := colind [[ (rowptr[row]) -- (rowptr[row + 1]) ]].
+Definition mind_seg (row : int) := mind [[ (mcrd[row]) -- (mcrd[row + 1]) ]].
 
-Hypothesis nodup_eachcol : forall x : int, 0 <= x < Nrow -> NoDup (colind_seg x).
+Hypothesis nodup_eachcol : forall x : int, 0 <= x < Nrow -> NoDup (mind_seg x).
 
 Tactic Notation "seclocal_solver" :=
   first [ assumption 
-    | rewrite -/(colind_seg _); now apply nodup_eachcol
-    | (* for rowptr[?] <= N *)
-      try rewrite -> len_colind; try rewrite -> len_mval; 
-      try rewrite <- rowptr_last; apply rowptr_weakly_sorted; math
-    | (* for 0 <= rowptr[?] *)
-      rewrite <- rowptr_first at 1; apply rowptr_weakly_sorted; math
-    | (* for 0 <= rowptr[i] <= rowptr[i + 1] *)
-      split; [ rewrite <- rowptr_first at 1 | ]; apply rowptr_weakly_sorted; math
-    | intros; eapply colind_leq, in_interval_list; now eauto
+    | rewrite -/(mind_seg _); now apply nodup_eachcol
+    | (* for mcrd[?] <= N *)
+      try rewrite -> len_mind; try rewrite -> len_mval; 
+      try rewrite <- mcrd_last; apply mcrd_weakly_sorted; math
+    | (* for 0 <= mcrd[?] *)
+      rewrite <- mcrd_first at 1; apply mcrd_weakly_sorted; math
+    | (* for 0 <= mcrd[i] <= mcrd[i + 1] *)
+      split; [ rewrite <- mcrd_first at 1 | ]; apply mcrd_weakly_sorted; math
+    | intros; eapply mind_leq, in_interval_list; now eauto
     | idtac ]; auto.
 
+(* Accessor function for CSR format. Similar to uCSR but encodings of each row are stored 
+  consecutively in the natural order *)
 Definition get := 
 <{
-  fun mval colind rowptr i j =>
-    let lb = read_array rowptr i in
+  fun mval mind mcrd i j =>
+    let lb = mcrd[i] in
     let i' = i + 1 in
-    let rb = read_array rowptr i' in
-      sv.get j colind mval lb rb
+    let rb = mcrd[i'] in
+      sv.get j mind mval lb rb
 }>.
 
+(* #5 from the table
+  Summation of all elements in sparse CSR matrix *)
 Definition sum := 
   <{
-  fun mval colind rowptr =>
+  fun mval mind mcrd =>
   let s = ref 0 in
   for i <- [0, Nrow] {
-    let lb = read_array rowptr i in
+    let lb = mcrd[i] in
     let i' = i + 1 in
-    let rb = read_array rowptr i' in
-    let x = sv.sum colind mval lb rb in 
+    let rb = mcrd[i'] in
+    let x = sv.sum mind mval lb rb in 
       s += x
   };
   ! s
@@ -90,26 +94,28 @@ Local Notation D := (labeled (int * int)).
 Definition eld := @LibWP.eld (int * int)%type.
 Coercion eld : D >-> Dom.
 
-Lemma sum_spec `{Inhab D} (x_mval x_colind x_rowptr : loc) : 
-  {{ arr(x_mval, mval)⟨1, (0,0)⟩ \*
-     arr(x_colind, colind)⟨1, (0,0)⟩ \*
-     arr(x_rowptr, rowptr)⟨1, (0,0)⟩ \*
-     (\*_(i <- `[0, Nrow] \x `[0, Ncol]) arr(x_mval, mval)⟨2, i⟩) \*
-     (\*_(i <- `[0, Nrow] \x `[0, Ncol]) arr(x_colind, colind)⟨2, i⟩) \*
-     (\*_(i <- `[0, Nrow] \x `[0, Ncol]) arr(x_rowptr, rowptr)⟨2, i⟩) }}
+
+(* Specification for `sum` *)
+Lemma sum_spec `{Inhab D} (m_val m_ind m_crd : loc) : 
+  {{ arr(m_val, mval)⟨1, (0,0)⟩ \*
+     arr(m_ind, mind)⟨1, (0,0)⟩ \*
+     arr(m_crd, mcrd)⟨1, (0,0)⟩ \*
+     (\*_(i <- `[0, Nrow] \x `[0, Ncol]) arr(m_val, mval)⟨2, i⟩) \*
+     (\*_(i <- `[0, Nrow] \x `[0, Ncol]) arr(m_ind, mind)⟨2, i⟩) \*
+     (\*_(i <- `[0, Nrow] \x `[0, Ncol]) arr(m_crd, mcrd)⟨2, i⟩) }}
   [{
-    [1| ld in `{(0,0)}   => sum x_mval x_colind x_rowptr];
-    {2| ld in `[0, Nrow] \x `[0, Ncol] => get x_mval x_colind x_rowptr ld.1 ld.2}
+    [1| ld in `{(0,0)}   => sum m_val m_ind m_crd];
+    {2| ld in `[0, Nrow] \x `[0, Ncol] => get m_val m_ind m_crd ld.1 ld.2}
   }]
   {{ hv, \[hv[`1]((0,0)) = Σ_(i <- `[0, Nrow] \x `[0, Ncol]) hv[`2](i)] \* \Top}}. (* this \Top can be made concrete, if needed *)
 Proof with (try seclocal_fold; seclocal_solver).
   xset_Inv Inv 1; xset_R Dom Inv R 2.
-  xin 2 : do 3 (xwp; xapp).
-  xin 1 : xwp; xapp=> s...
+  xin 2 : xgo.
+  xin 1 : xstep=> s...
   rewrite prod_cascade.
   xfor_sum Inv R R (fun hv i => Σ_(j <- `{i} \x `[0, Ncol]) hv[`2](j)) s.
   { xin 2 : rewrite wp_prod_single /=.
-    xin 1 : do 3 (xwp; xapp)...
+    xin 1 : do 3 xtep...
     xsubst (snd : _ -> int).
     xnapp sv.sum_spec...
     xsimpl=>->. xapp @incr.spec; rewrite sum_prod1E; xsimpl. }
@@ -119,44 +125,48 @@ Qed.
 Context (dvec : list int).
 Context (dvec_len : length dvec = Ncol :> int).
 
+
+(* #6 from the table
+  Dot product of a sparse CSR matrix and a dense vector *)
 Definition spmv := 
   <{
-  fun mval colind rowptr dvec =>
+  fun mval mind mcrd dvec =>
   let s = alloc0 Nrow in
   for i <- [0, Nrow] {
-    let lb = read_array rowptr i in
+    let lb = mcrd[i] in
     let i' = i + 1 in
-    let rb = read_array rowptr i' in
-    let x = sv.dotprod colind mval dvec lb rb in 
-    val_array_set s i x
+    let rb = mcrd[i'] in
+    let x = sv.dotprod mind mval dvec lb rb in 
+    s[i] := x
   }; 
   s
 }>.
 
-Lemma spmv_spec `{Inhab D} (x_mval x_colind x_rowptr x_dvec : loc) : 
-  {{ arr(x_mval, mval)⟨1, (0,0)⟩ \*
-     arr(x_colind, colind)⟨1, (0,0)⟩ \*
-     arr(x_rowptr, rowptr)⟨1, (0,0)⟩ \*
+(* Specification for `spmv` *)
+Lemma spmv_spec `{Inhab D} (m_val m_ind m_crd x_dvec : loc) : 
+  {{ arr(m_val, mval)⟨1, (0,0)⟩ \*
+     arr(m_ind, mind)⟨1, (0,0)⟩ \*
+     arr(m_crd, mcrd)⟨1, (0,0)⟩ \*
      arr(x_dvec, dvec)⟨1, (0,0)⟩ \* 
-     (\*_(i <- `[0, Nrow] \x `[0, Ncol]) arr(x_mval, mval)⟨2, i⟩) \*
-     (\*_(i <- `[0, Nrow] \x `[0, Ncol]) arr(x_colind, colind)⟨2, i⟩) \*
-     (\*_(i <- `[0, Nrow] \x `[0, Ncol]) arr(x_rowptr, rowptr)⟨2, i⟩) \*
+     (\*_(i <- `[0, Nrow] \x `[0, Ncol]) arr(m_val, mval)⟨2, i⟩) \*
+     (\*_(i <- `[0, Nrow] \x `[0, Ncol]) arr(m_ind, mind)⟨2, i⟩) \*
+     (\*_(i <- `[0, Nrow] \x `[0, Ncol]) arr(m_crd, mcrd)⟨2, i⟩) \*
      (\*_(i <- `[0, Nrow] \x `[0, Ncol]) arr(x_dvec, dvec)⟨2, i⟩) }}
   [{
-    [1| ld in `{(0,0)}                 => spmv x_mval x_colind x_rowptr x_dvec];
-    {2| ld in `[0, Nrow] \x `[0, Ncol] => get x_mval x_colind x_rowptr ld.1 ld.2}
+    [1| ld in `{(0,0)}                 => spmv m_val m_ind m_crd x_dvec];
+    {2| ld in `[0, Nrow] \x `[0, Ncol] => get m_val m_ind m_crd ld.1 ld.2}
   }]
   {{ hv, 
     harray_fun_int (fun i => Σ_(j <- `[0, Ncol]) hv[`2]((i, j)) * dvec[j]) (hv[`1]((0,0))) Nrow (Lab (1,0) (0,0))
       \* \Top }}. (* this \Top can be made concrete, if needed *)
 Proof with (try seclocal_fold; seclocal_solver).
   xset_Inv Inv 1; xset_R Dom Inv R 2.
-  xin 2 : do 3 (xwp; xapp).
+  xin 2 : xgo.
   xin 1 : (xwp; xapp (@htriple_alloc0_unary)=> // s)...
   rewrite prod_cascade.
   xfor_arrayset Inv R R (fun hv (i : int) => Σ_(j <- `{i} \x `[0, Ncol]) (hv[`2](j) * dvec[j.2])) (fun _ : int => 0) s.
   { xin 2 : rewrite wp_prod_single /=.
-    xin 1 : do 3 (xwp; xapp)...
+    xin 1 : xgo...
     xsubst (snd : _ -> int).
     xnapp sv.dotprod_spec...
     xsimpl=>->. xapp @lhtriple_array_set_pre; try math.
@@ -173,39 +183,41 @@ Hypothesis yind_leq : forall x, In x yind -> 0 <= x < Ncol.
 Hypothesis Nrow0 : Nrow > 0. (* we get rid of it later *)
 
 
-Hypothesis sorted_eachcol : forall x : int, 0 <= x < Nrow -> sorted (colind_seg x).
+Hypothesis sorted_eachcol : forall x : int, 0 <= x < Nrow -> sorted (mind_seg x).
 
-Definition spmspv x_colind y_ind x_mval y_val := 
-  let dot := sv.sv_dotprod x_colind y_ind x_mval y_val in
+(* #7 from the table
+  Product of sparse CSR matrix and sparse SV vector *)
+Definition spmspv m_ind y_ind m_val y_val := 
+  let dot := sv.sv_dotprod m_ind y_ind m_val y_val in
   <{
-  fun rowptr =>
+  fun mcrd =>
   let s = alloc0 Nrow in
   for i <- [0, Nrow] {
-    let lb = read_array rowptr i in
+    let lb = mcrd[i] in
     let i' = i + 1 in
-    let rb = read_array rowptr i' in
+    let rb = mcrd[i'] in
     let x = dot lb rb 0 M in 
-      val_array_set s i x
+      s[i] := x
   }; 
   s
 }>.
 
-
+(* Specification for `spmspv` *)
 Lemma spmspv_spec `{Inhab D}
-  (x_mval x_colind x_rowptr y_ind y_val : loc) : 
-  {{ arr(x_mval, mval)⟨1, (0,0)⟩ \*
-     arr(x_colind, colind)⟨1, (0,0)⟩ \*
-     arr(x_rowptr, rowptr)⟨1, (0,0)⟩ \*
+  (m_val m_ind m_crd y_ind y_val : loc) : 
+  {{ arr(m_val, mval)⟨1, (0,0)⟩ \*
+     arr(m_ind, mind)⟨1, (0,0)⟩ \*
+     arr(m_crd, mcrd)⟨1, (0,0)⟩ \*
      arr(y_ind, yind)⟨1, (0,0)⟩ \* 
      arr(y_val, yval)⟨1, (0,0)⟩ \* 
-     (\*_(i <- `[0, Nrow] \x `[0, Ncol]) arr(x_mval, mval)⟨2, i⟩) \*
-     (\*_(i <- `[0, Nrow] \x `[0, Ncol]) arr(x_colind, colind)⟨2, i⟩) \*
-     (\*_(i <- `[0, Nrow] \x `[0, Ncol]) arr(x_rowptr, rowptr)⟨2, i⟩) \*
+     (\*_(i <- `[0, Nrow] \x `[0, Ncol]) arr(m_val, mval)⟨2, i⟩) \*
+     (\*_(i <- `[0, Nrow] \x `[0, Ncol]) arr(m_ind, mind)⟨2, i⟩) \*
+     (\*_(i <- `[0, Nrow] \x `[0, Ncol]) arr(m_crd, mcrd)⟨2, i⟩) \*
      (\*_(i <- `{0} \x `[0, Ncol]) arr(y_ind, yind)⟨3, i⟩) \* 
      (\*_(i <- `{0} \x `[0, Ncol]) arr(y_val, yval)⟨3, i⟩) }}
   [{
-    {1| ld in `{(0,0)}                 => spmspv x_colind y_ind x_mval y_val x_rowptr};
-    {2| ld in `[0, Nrow] \x `[0, Ncol] => get x_mval x_colind x_rowptr ld.1 ld.2};
+    {1| ld in `{(0,0)}                 => spmspv m_ind y_ind m_val y_val m_crd};
+    {2| ld in `[0, Nrow] \x `[0, Ncol] => get m_val m_ind m_crd ld.1 ld.2};
     {3| ld in `{0}       \x `[0, Ncol] => sv.get ld.2 y_ind y_val 0 M}
   }]
   {{ hv,
@@ -213,13 +225,13 @@ Lemma spmspv_spec `{Inhab D}
       \* \Top }}. (* this \Top can be made concrete, if needed *)
 Proof with (try seclocal_fold; seclocal_solver; try lia).
   xset_Inv Inv 1; xset_R_core Dom R1 2; xset_R_core Dom R2 3. xset_clean R1 R2 Inv.
-  xin 2 : do 3 (xwp; xapp).
+  xin 2 : xgo.
   xin 1 : (xwp; xapp (@htriple_alloc0_unary)=> // s)...
   rewrite prod_cascade -(Union_same Nrow (`{0} \x `[0, Ncol])) //; try math.
   xfor_arrayset Inv R1 R1 R2 R2 
     (fun hv (i : int) => Σ_(j <- `{i} \x `[0, Ncol]) (hv[`2](j) * hv[`3]((0, j.2)))) (fun _ : int => 0) s.
   { xin 2 : rewrite wp_prod_single /=.
-    xin 1 : do 3 (xwp; xapp)...
+    xin 1 : xgo...
     xsubst (snd : _ -> int).
     xnapp @sv.sv_dotprod_spec... 
     { by rewrite -len_xind slice_fullE. }
