experiments/uCSR.v
@@ -16,8 +16,8 @@ Section unordered_csr.
 
 Notation "'mval'" := ("m_val":var) (in custom trm at level 0) : trm_scope.
 Notation "'midx'" := ("m_idx":var) (in custom trm at level 0) : trm_scope.
-Notation "'colind'" := ("col_ind":var) (in custom trm at level 0) : trm_scope.
-Notation "'rowptr'" := ("row_ptr":var) (in custom trm at level 0) : trm_scope.
+Notation "'mind'" := ("m_ind":var) (in custom trm at level 0) : trm_scope.
+Notation "'mcrd'" := ("m_crd":var) (in custom trm at level 0) : trm_scope.
 Notation "'dvec'" := ("d_vec":var) (in custom trm at level 0) : trm_scope.
 Notation "'lb'" := ("l_b":var) (in custom trm at level 0) : trm_scope.
 Notation "'rb'" := ("r_b":var) (in custom trm at level 0) : trm_scope.
@@ -25,23 +25,23 @@ Notation "'i''" := ("i_'":var) (in custom trm at level 0) : trm_scope.
 
 Import List Vars list_interval_notation.
 
-Context (mval midx colind rowptr : list int).
+Context (mval midx mind mcrd : list int).
 Context (N Nrow Ncol Nidx : int).
 Hypothesis Nrow_nonneg : 0 <= Nrow.
 Hypothesis len_mval : length mval = N :> int.
 Hypothesis len_midx : length midx = Nidx :> int.
 Hypotheses Nidx_leq_Nrow : Nidx <= Nrow.
-Hypothesis len_colind : length colind = N :> int.
-Hypothesis len_rowptr : length rowptr = Nidx + 1 :> int.
-Hypothesis colind_leq : forall x, In x colind -> 0 <= x < Ncol.
+Hypothesis len_mind : length mind = N :> int.
+Hypothesis len_mcrd : length mcrd = Nidx + 1 :> int.
+Hypothesis mind_leq : forall x, In x mind -> 0 <= x < Ncol.
 Hypothesis midx_leq : forall x, In x midx -> 0 <= x < Nrow.
-Hypothesis rowptr_first : rowptr[0] = 0.
-Hypothesis rowptr_last : rowptr[Nidx] = N.
-Hypothesis rowptr_weakly_sorted : forall (i j : int), 
+Hypothesis mcrd_first : mcrd[0] = 0.
+Hypothesis mcrd_last : mcrd[Nidx] = N.
+Hypothesis mcrd_weakly_sorted : forall (i j : int), 
   (0 <= i <= Nidx) -> 
   (0 <= j <= Nidx) -> 
   (i <= j) -> 
-  (rowptr[i] <= rowptr[j]).
+  (mcrd[i] <= mcrd[j]).
 
 Context (yind yval : list int).
 Context (M : int).
@@ -51,23 +51,23 @@ Hypothesis stored_yind : sorted yind.
 Hypothesis yind_leq : forall x, In x yind -> 0 <= x < Ncol.
 Hypothesis Nrow0 : Nidx > 0. (* we get rid of it later *)
 
-Definition colind_seg (row : int) := colind [[ (rowptr[row]) -- (rowptr[row + 1]) ]].
+Definition mind_seg (row : int) := mind [[ (mcrd[row]) -- (mcrd[row + 1]) ]].
 
-Hypothesis nodup_eachcol : forall x : int, 0 <= x < Nidx -> NoDup (colind_seg x).
+Hypothesis nodup_eachcol : forall x : int, 0 <= x < Nidx -> NoDup (mind_seg x).
 Hypotheses nodup_midx : NoDup midx.
 
 Tactic Notation "seclocal_solver" :=
   try (rewrite index_nodup=> //; math);
   first [ assumption 
-    | rewrite -/(colind_seg _); now apply nodup_eachcol
-    | (* for rowptr[?] <= N *)
-      try rewrite -> len_colind; try rewrite -> len_mval; 
-      try rewrite <- rowptr_last; apply rowptr_weakly_sorted; math
-    | (* for 0 <= rowptr[?] *)
-      rewrite <- rowptr_first at 1; apply rowptr_weakly_sorted; math
-    | (* for 0 <= rowptr[i] <= rowptr[i + 1] *)
-      split; [ rewrite <- rowptr_first at 1 | ]; apply rowptr_weakly_sorted; math
-    | intros; eapply colind_leq, in_interval_list; now eauto
+    | rewrite -/(mind_seg _); now apply nodup_eachcol
+    | (* for mcrd[?] <= N *)
+      try rewrite -> len_mind; try rewrite -> len_mval; 
+      try rewrite <- mcrd_last; apply mcrd_weakly_sorted; math
+    | (* for 0 <= mcrd[?] *)
+      rewrite <- mcrd_first at 1; apply mcrd_weakly_sorted; math
+    | (* for 0 <= mcrd[i] <= mcrd[i + 1] *)
+      split; [ rewrite <- mcrd_first at 1 | ]; apply mcrd_weakly_sorted; math
+    | intros; eapply mind_leq, in_interval_list; now eauto
     | intros; now case_if
     | move=> >; rewrite -len_xind slice_fullE //
     | lia
@@ -76,206 +76,103 @@ Tactic Notation "seclocal_solver" :=
 
 Definition indexf := index.func Nidx.
 
-Definition get (x_mval : loc) := 
+
+(* Accessor function for uCSR format. Similar to `ucsr_get` in  Fig.2.c from the paper. 
+  This encoding is a "real-world" version of the one presented in a paper. Instead of 
+  storing the encoding of each row of the matrix as elements of two-dimensional arrays
+  `mval` and `mind`, we concatenate them into one-dimensional arrays `mval` and `mind`
+  and store an additional array `mcrd` wich says where does the eancoding of each 
+  new row starts. Using this encoding the example from Fig.2.a can be represented as follows:
+   
+  midx :  [3, 0, 4, 3]
+  
+  mcrd: [0, 1,    3, 4,   6]
+  mind:  [2, 1, 4, 4, 1, 3]
+  mval:  [C, A, B, G, D, E] *)
+Definition get (m_val : loc) := 
 <{
-  fun midx colind rowptr i j =>
+  fun midx mind mcrd i j =>
       let i = indexf i midx in
       let "i < Nidx" = i < Nidx in
       if "i < Nidx" then
-        let lb = read_array rowptr i in
+        let lb = mcrd[i] in
         let i' = i + 1 in
-        let rb = read_array rowptr i' in
-          sv.get j colind x_mval lb rb
+        let rb = mcrd[i'] in
+          sv.get j mind m_val lb rb
       else 0
 }>.
 
-Lemma get_spec_out_unary {D : Type} `{Inhab D} (x_midx x_mval x_colind x_rowptr : loc) (i j : int) d :
-  @htriple D (single d tt) 
-    (fun=> get x_mval x_midx x_colind x_rowptr i j)
-    (\[~ In i midx] \*
-      harray_int mval x_mval d \* 
-      harray_int midx x_midx d \* 
-      harray_int colind x_colind d \* 
-      harray_int rowptr x_rowptr d)
+(* Unary specification for `ucsr_get` called outside of the `midx` array. 
+  Generalised version of eq. (8) from the paper *)
+Lemma get_spec_out_unary {D : Type} `{Inhab D} (m_idx m_val m_ind m_crd : loc) (i j : int) (d : D) :
+  htriple (`{d}) (* The index set here is just an arbitrary singleton set `{d}` *)
+    (fun=> get m_val m_idx m_ind m_crd i j) (* We run out `get` funtion on indicies `i` and `j` *)
+    (\[~ In i midx] \*                      (* such that `i` ∉ midx *)
+      arr(m_val, mval)⟨`d⟩ \* 
+      arr(m_idx, midx)⟨`d⟩ \* 
+      arr(m_ind, mind)⟨`d⟩ \* 
+      arr(m_crd, mcrd)⟨`d⟩)
     (fun hr => 
-     \[hr = fun=> 0] \* 
-      harray_int mval x_mval d \* 
-      harray_int midx x_midx d \* 
-      harray_int colind x_colind d \* 
-      harray_int rowptr x_rowptr d).
+     \[hr = fun=> 0] \* (* the output is the singleton hyper-value indexed by `{d}`, which is equal to 0 *)
+      arr(m_val, mval)⟨`d⟩ \* 
+      arr(m_idx, midx)⟨`d⟩ \* 
+      arr(m_ind, mind)⟨`d⟩ \* 
+      arr(m_crd, mcrd)⟨`d⟩).
 Proof with seclocal_solver.
-  xwp; xsimpl=> /(memNindex _)?; xapp @index.spec... 
-  xstep; xwp; xif=> ?... 
-  xwp; xval; xsimpl*.
+  xwp; xsimpl=> /(memNindex _)?; xapp @index.spec... (* apply index function specification *) 
+  xstep; xwp; xif=> ?... (* case analysis on `i < Nidx` condition *)
+  xwp; xval; xsimpl*. (* finish the proof *)
 Qed.
 
-Lemma get_spec_out `{Inhab (labeled (int * int))} fs (x_midx x_mval x_colind x_rowptr : loc) : 
-  @htriple (labeled (int * int)) fs
-    (fun d => get x_mval x_midx x_colind x_rowptr (eld d).1 (eld d).2)
-    (\[forall d, indom fs d -> ~ In (eld d).1 midx] \*
-      (\*_(d <- fs) harray_int mval x_mval d) \* 
-      (\*_(d <- fs) harray_int midx x_midx d) \* 
-      (\*_(d <- fs) harray_int colind x_colind d) \* 
-       \*_(d <- fs) harray_int rowptr x_rowptr d)
+
+Local Notation Dom := (int * int)%type.
+Local Notation D := (labeled (int * int)).
+Definition get_index := @LibWP.eld (int * int)%type.
+Coercion get_index : D >-> Dom. (* `get_index` is a coercion of `labeled (int * int)` to `int * int` *)
+
+(* Hyper specification for `ucsr_get` function, called on a set of indecies,
+  outside of the `midx` array. The index set in this case is a finite 
+  set (`fset`) of elements `⟨l, i, j⟩` with type `labeled (int * int)`.
+  Generalised version of eq.(7) from the paper. *)
+Lemma get_spec_out `{Inhab (labeled (int * int))} (fs : fset (labeled (int * int))) (m_idx m_val m_ind m_crd : loc) : 
+  htriple fs
+    (fun ij => get m_val m_idx m_ind m_crd ij.1 ij.2) 
+    (\[forall d, indom fs d -> ~ In (get_index d).1 midx] \* (* for all `⟨l, i, j⟩` elements of `fs`, `i ∉ midx` *)
+      (\*_(d <- fs) arr(m_val, mval)⟨`d⟩) \* 
+      (\*_(d <- fs) arr(m_idx, midx)⟨`d⟩) \* 
+      (\*_(d <- fs) arr(m_ind, mind)⟨`d⟩) \* 
+       \*_(d <- fs) arr(m_crd, mcrd)⟨`d⟩)
     (fun hr => 
      \[hr = fun=> 0] \* 
-      (\*_(d <- fs) harray_int mval x_mval d) \*
-      (\*_(d <- fs) harray_int midx x_midx d) \* 
-      (\*_(d <- fs) harray_int colind x_colind d) \*  
-       \*_(d <- fs) harray_int rowptr x_rowptr d).
-Proof. by xpointwise_build (@get_spec_out_unary). Qed.
+      (\*_(d <- fs) arr(m_val, mval)⟨`d⟩) \*
+      (\*_(d <- fs) arr(m_idx, midx)⟨`d⟩) \* 
+      (\*_(d <- fs) arr(m_ind, mind)⟨`d⟩) \*  
+       \*_(d <- fs) arr(m_crd, mcrd)⟨`d⟩).
+Proof. by xpointwise_build (@get_spec_out_unary). Qed. (* apply `Product` rule from Fig. 4 *)
 
-Definition sum := 
-  <{
-    fun mval midx colind rowptr =>
-    let s = ref 0 in
-    for i <- [0, Nidx] {
-      let lb = read_array rowptr i in
-      let i' = i + 1 in
-      let rb = read_array rowptr i' in
-      let x = sv.sum colind mval lb rb in 
-        s += x
-    };
-    ! s
-}>.
 
 Tactic Notation "seclocal_fold" := 
   rewrite ?label_single ?wp_single
     -/(For_aux _ _) 
     -/(For _ _ _) //=.
 
-Local Notation Dom := (int * int)%type.
-Local Notation D := (labeled (int * int)).
-Definition eld := @LibWP.eld (int * int)%type.
-Coercion eld : D >-> Dom.
 
-Lemma sum_spec `{Inhab D} `{Inhab (labeled int)} (x_mval x_colind x_rowptr x_midx : loc) : 
-  {{ arr(x_mval, mval)⟨1, (0,0)⟩ \*
-     arr(x_midx, midx)⟨1, (0,0)⟩ \*
-     arr(x_colind, colind)⟨1, (0,0)⟩ \*
-     arr(x_rowptr, rowptr)⟨1, (0,0)⟩ \*
-     (\*_(i <- `[0, Nrow] \x `[0, Ncol]) arr(x_mval, mval)⟨2, i⟩) \*
-     (\*_(i <- `[0, Nrow] \x `[0, Ncol]) arr(x_midx, midx)⟨2, i⟩) \*
-     (\*_(i <- `[0, Nrow] \x `[0, Ncol]) arr(x_colind, colind)⟨2, i⟩) \*
-     (\*_(i <- `[0, Nrow] \x `[0, Ncol]) arr(x_rowptr, rowptr)⟨2, i⟩) }}
-  [{
-    [1| ld in `{(0,0)}   => sum x_mval x_midx x_colind x_rowptr];
-    {2| ld in `[0, Nrow] \x `[0, Ncol] => get x_mval x_midx x_colind x_rowptr ld.1 ld.2}
-  }]
-  {{ hv, \[hv[`1]((0,0)) = Σ_(i <- `[0, Nrow] \x `[0, Ncol]) hv[`2](i)] \* \Top}}.
-Proof with (try seclocal_fold; seclocal_solver).
-  xset_Inv Inv 1; xset_R int Inv R 2.
-  xfocus* 2 (indom (midx \x `[0, Ncol])).
-  xapp get_spec_out=> //. 1: case=> ??; indomE; tauto.
-  xclean_heap.
-  have E : (`[0, Nrow] \x `[0, Ncol]) ∩ indom (midx \x `[0, Ncol]) = midx \x `[0, Ncol].
-  { rewrite -prod_intr_list_on_1. f_equal. now apply intr_list. }
-  rewrite E (fset_of_list_nodup 0 nodup_midx) len_midx prod_Union_distr.
-  xin 1 : xwp; xapp=> s...
-  xfor_sum Inv R R (fun hv i => Σ_(j <- `{midx[i]} \x `[0, Ncol]) hv[`2](j)) s.
-  { xin 2 : rewrite wp_prod_single /=.
-    xin 1 : do 3 (xwp; xapp)...
-    xsubst (snd : _ -> int).
-    xfocus (2,0); rewrite -> ! hbig_fset_hstar.
-    xwp; xapp (@index.Spec `[0, Ncol] Nidx (2,0) midx x_midx (fun=> midx[l0]))=> //.
-    rewrite index_nodup //; try math.
-    xwp; xapp. xwp; xif=> ?; [ | math ].
-    do 3 (xwp; xapp).
-    xunfocus; xin 1 : idtac. (* reformat *)
-    xnapp sv.sum_spec...
-    xsimpl=>->. xapp @incr.spec. rewrite sum_prod1E. xsimpl. }
-  { move=>Ha Hb Hc; left. move: Ha; apply contrapose, NoDup_nthZ; autos*; math. }
-  xwp; xapp. xsimpl*. xsum_normalize.
-  rewrite SumCascade -?prod_Union_distr -?len_midx -?(fset_of_list_nodup 0) ?E //.
-  disjointE.
-  move=>Ha Hb Hc; left. move: Ha; apply contrapose, NoDup_nthZ; autos*; math.
-Qed.
+Hypothesis sorted_eachcol : forall x : int, 0 <= x < Nidx -> sorted (mind_seg x).
 
-Context (dvec : list int).
-Context (dvec_len : length dvec = Ncol :> int).
-
-(* challenge: unordered array set *)
-Definition spmv := 
+(* #10 from the table
+  Version of `spmspv` from Fig.3 *)
+Definition spmspv m_ind y_ind m_val y_val := 
+  let spvspv := sv.sv_dotprod m_ind y_ind m_val y_val in
   <{
-  fun mval midx colind rowptr dvec =>
+  fun mcrd midx =>
   let s = alloc0 Nrow in
   for i <- [0, Nidx] {
-    let lb = read_array rowptr i in
+    let lb = mcrd[i] in
     let i' = i + 1 in
-    let rb = read_array rowptr i' in
-    let i = read_array midx i in
-    let x = sv.dotprod colind mval dvec lb rb in 
-    val_array_set s i x
-  }; 
-  s
-}>.
-
-Lemma spmv_spec `{Inhab D} `{H__ : Inhab (labeled int)} (x_mval x_midx x_colind x_rowptr x_dvec : loc) : 
-  {{ arr(x_mval, mval)⟨1, (0,0)⟩ \*
-     arr(x_midx, midx)⟨1, (0,0)⟩ \*
-     arr(x_colind, colind)⟨1, (0,0)⟩ \*
-     arr(x_rowptr, rowptr)⟨1, (0,0)⟩ \*
-     arr(x_dvec, dvec)⟨1, (0,0)⟩ \* 
-     (\*_(i <- `[0, Nrow] \x `[0, Ncol]) arr(x_mval, mval)⟨2, i⟩) \*
-     (\*_(i <- `[0, Nrow] \x `[0, Ncol]) arr(x_midx, midx)⟨2, i⟩) \*
-     (\*_(i <- `[0, Nrow] \x `[0, Ncol]) arr(x_colind, colind)⟨2, i⟩) \*
-     (\*_(i <- `[0, Nrow] \x `[0, Ncol]) arr(x_rowptr, rowptr)⟨2, i⟩) \*
-     (\*_(i <- `[0, Nrow] \x `[0, Ncol]) arr(x_dvec, dvec)⟨2, i⟩) }}
-  [{
-    [1| ld in `{(0,0)}                 => spmv x_mval x_midx x_colind x_rowptr x_dvec];
-    {2| ld in `[0, Nrow] \x `[0, Ncol] => get x_mval x_midx x_colind x_rowptr ld.1 ld.2}
-  }]
-  {{ hv,
-    harray_fun_int (fun i => Σ_(j <- `[0, Ncol]) hv[`2]((i, j)) * dvec[j]) (hv[`1]((0,0))) Nrow (Lab (1,0) (0,0))
-      \* \Top }}.
-Proof with (try seclocal_fold; seclocal_solver).
-  xset_Inv Inv 1; xset_R int Inv R 2.
-  xfocus* 2 (indom (midx \x `[0, Ncol])).
-  xapp get_spec_out=> //. 1: case=> ??; indomE; tauto.
-  xclean_heap.
-  have E : (`[0, Nrow] \x `[0, Ncol]) ∩ indom (midx \x `[0, Ncol]) = midx \x `[0, Ncol].
-  { rewrite -prod_intr_list_on_1. f_equal. now apply intr_list. }
-  rewrite E (fset_of_list_nodup 0 nodup_midx) len_midx prod_Union_distr.
-  xin 1 : xmalloc ans...
-  xfor_arrayset Inv R R 
-    (fun hv (i : int) => (If (In i midx) then Σ_(j <- `{i} \x `[0, Ncol]) (hv[`2](j) * dvec[j.2]) else 0)) 
-    (fun _ : int => 0) ans midx...
-  { xin* 2: xapp* @index.specs; xstep; xwp; xif=> [?|]; xgo...
-    xin 1 : xgo...
-    rewrite index_nodup //; try math.
-    xsubst (snd : _ -> int).
-    xnapp sv.dotprod_spec...
-    xsimpl=>->; xapp; rewrite sum_prod1E; xsimpl.
-    case: classicT=> [?|/(_ (nth_In _ _ _))] //; lia. }
-  xwp; xval. xsimpl*. erewrite -> harray_fun_int_congr; try assumption; first xsimpl*.
-  move=> i Hi /=. xsum_normalize.
-  case_if.
-  { rewrite sum_prod1E /=; apply SumEq=> >; indomE.
-    case: classicT=> // /[swap]? []; exists (index i midx); indomE=> /=.
-    splits; try tauto. 
-    { rewrite -len_midx index_mem //; splits*; exact/(indexG0). }
-    { by rewrite nth_index. } }
-  { rewrite -> SumEq with (G:=fun=> 0)=> [|?]; first by rewrite Sum0s.
-    indomE; case: classicT=> // -[?]; indomE=> /=-[?][*]. 
-    case: C; subst; apply/nth_In; math. }
-Qed.
-
-
-
-Hypothesis sorted_eachcol : forall x : int, 0 <= x < Nidx -> sorted (colind_seg x).
-
-Definition spmspv x_colind y_ind x_mval y_val := 
-  let dot := sv.sv_dotprod x_colind y_ind x_mval y_val in
-  <{
-  fun rowptr midx =>
-  let s = alloc0 Nrow in
-  for i <- [0, Nidx] {
-    let lb = read_array rowptr i in
-    let i' = i + 1 in
-    let rb = read_array rowptr i' in
-    let i = read_array midx i in
-    let x = dot lb rb 0 M in 
-      val_array_set s i x
+    let rb = mcrd[i'] in
+    let i = midx[i] in
+    let x = spvspv lb rb 0 M in 
+      s[i] := x
   }; 
   s
 }>.
@@ -286,41 +183,31 @@ Notation size := length.
 (*********  The full verison of the proof snippet from Section 4 of the paper *********)
 (**************************************************************************************)
 (* 
-  Major differencies with the paper verison: 
-  (1) Our Coq implementation only supports LGTM triples, where index sets of all 
-    components have the same type. To run the `uscr_get` funtion (`get` here) we need an
-    index set with elements of type `int * int`. That is why indexs sets of the first 
-    and the third components are artifically made to have the same type as well. 
-  (2) Instread `xfor` tactic from the paper, we use a more convinient tactic 
-    `xfor_bigstr`. This tactic takes not the whole invariant as an input, but only that
-    part of it, which changes within the inductive step. Here we provide it some
-    technical arguments `Inv`, `R2`, `R3`, althother with two verisions of the changed 
-    clause from I_for: before and after the induvtive step.
-  (3) The Coq notation for `x(i) |-> y` heap predicate is `x |-(i)-> y`. 
-  (4) The Coq notation for `arr(x(i), y)` heap predicate is `arr(x, y)⟨i⟩`. 
-  (5) In the paper the output of each component is a separate hyper vaule. Here all 
-    outputs are assembled in the same hyper value `hv`. To reference to the outcome of
-    each particular componet with tag `t`, one should write `hv[`t]`.
+  Instead of `xfor` tactic from the paper, we use a more convenient tactic 
+  `xfor_bigstr`. This tactic takes not the whole invariant as an input, but only that
+  part of it, which changes within the inductive step. Here we provide it some
+  technical arguments `Inv`, `R2`, `R3`, althother with two verisions of the changed 
+  clause from I_for: before and after the inductive step.
 *)
 
 Lemma spmspv_spec `{Inhab D} `{H__ : Inhab (labeled int)}
-  (x_mval x_colind x_midx x_rowptr y_ind y_val : loc) : 
-  {{ arr(x_mval, mval)⟨1, (0,0)⟩ \*
-     arr(x_midx, midx)⟨1, (0,0)⟩ \*
-     arr(x_colind, colind)⟨1, (0,0)⟩ \*
-     arr(x_rowptr, rowptr)⟨1, (0,0)⟩ \*
+  (m_val m_ind m_idx m_crd y_ind y_val : loc) : 
+  {{ arr(m_val, mval)⟨1, (0,0)⟩ \*
+     arr(m_idx, midx)⟨1, (0,0)⟩ \*
+     arr(m_ind, mind)⟨1, (0,0)⟩ \*
+     arr(m_crd, mcrd)⟨1, (0,0)⟩ \*
      arr(y_ind, yind)⟨1, (0,0)⟩ \* 
      arr(y_val, yval)⟨1, (0,0)⟩ \* 
-     (\*_(i <- `[0, Nrow] \x `[0, Ncol]) arr(x_mval, mval)⟨2, i⟩) \*
-     (\*_(i <- `[0, Nrow] \x `[0, Ncol]) arr(x_midx, midx)⟨2, i⟩) \*
-     (\*_(i <- `[0, Nrow] \x `[0, Ncol]) arr(x_colind, colind)⟨2, i⟩) \*
-     (\*_(i <- `[0, Nrow] \x `[0, Ncol]) arr(x_rowptr, rowptr)⟨2, i⟩) \*
+     (\*_(i <- `[0, Nrow] \x `[0, Ncol]) arr(m_val, mval)⟨2, i⟩) \*
+     (\*_(i <- `[0, Nrow] \x `[0, Ncol]) arr(m_idx, midx)⟨2, i⟩) \*
+     (\*_(i <- `[0, Nrow] \x `[0, Ncol]) arr(m_ind, mind)⟨2, i⟩) \*
+     (\*_(i <- `[0, Nrow] \x `[0, Ncol]) arr(m_crd, mcrd)⟨2, i⟩) \*
      (\*_(i <- `{0} \x `[0, Ncol]) arr(y_ind, yind)⟨3, i⟩) \* 
      (\*_(i <- `{0} \x `[0, Ncol]) arr(y_val, yval)⟨3, i⟩) }}
   [{
-    {1| ld in `{(0,0)}                 => spmspv x_colind y_ind x_mval y_val x_rowptr x_midx};
-    {2| ld in `[0, Nrow] \x `[0, Ncol] => get x_mval x_midx x_colind x_rowptr ld.1 ld.2};
-    {3| ld in `{0}       \x `[0, Ncol] => sv.get ld.2 y_ind y_val 0 M}
+    {1| _  in `{(0,0)}                 => spmspv m_ind y_ind m_val y_val m_crd m_idx};
+    {2| ij in `[0, Nrow] \x `[0, Ncol] => get m_val m_idx m_ind m_crd ij.1 ij.2};
+    {3| zj in `{0}       \x `[0, Ncol] => sv.get zj.2 y_ind y_val 0 M}
   }]
   {{ hv,
     arrf(hv[`1]((0,0)), i in Nrow => Σ_(j <- `[0, Ncol]) hv[`2]((i, j)) * hv[`3]((0, j)))⟨1, (0,0)⟩
@@ -361,6 +248,131 @@ Proof with (try seclocal_fold; seclocal_solver; autos* ).
   rewrite -prod_Union_distr -len_midx -fset_of_list_nodup; indomE=> //=.
   rewrite -index_mem index_nodup; try case_if...
 Qed. 
+
+(* #8 from the table
+  Summation of all elements in uCSR sparse maitrix *)
+Definition sum := 
+  <{
+    fun mval midx mind mcrd =>
+    let s = ref 0 in
+    for i <- [0, Nidx] {
+      let lb = mcrd[i] in
+      let i' = i + 1 in
+      let rb = mcrd[i'] in
+      let x = sv.sum mind mval lb rb in 
+        s += x
+    };
+    ! s
+}>.
+
+(* Specification for `sum` *)
+Lemma sum_spec `{Inhab D} `{Inhab (labeled int)} (m_val m_ind m_crd m_idx : loc) : 
+  {{ arr(m_val, mval)⟨1, (0,0)⟩ \*
+     arr(m_idx, midx)⟨1, (0,0)⟩ \*
+     arr(m_ind, mind)⟨1, (0,0)⟩ \*
+     arr(m_crd, mcrd)⟨1, (0,0)⟩ \*
+     (\*_(i <- `[0, Nrow] \x `[0, Ncol]) arr(m_val, mval)⟨2, i⟩) \*
+     (\*_(i <- `[0, Nrow] \x `[0, Ncol]) arr(m_idx, midx)⟨2, i⟩) \*
+     (\*_(i <- `[0, Nrow] \x `[0, Ncol]) arr(m_ind, mind)⟨2, i⟩) \*
+     (\*_(i <- `[0, Nrow] \x `[0, Ncol]) arr(m_crd, mcrd)⟨2, i⟩) }}
+  [{
+    [1| _  in `{(0,0)}   => sum m_val m_idx m_ind m_crd];
+    {2| ij in `[0, Nrow] \x `[0, Ncol] => get m_val m_idx m_ind m_crd ij.1 ij.2}
+  }]
+  {{ hv, \[hv[`1]((0,0)) = Σ_(i <- `[0, Nrow] \x `[0, Ncol]) hv[`2](i)] \* \Top}}.
+Proof with (try seclocal_fold; seclocal_solver).
+  xset_Inv Inv 1; xset_R int Inv R 2. (* start the proof *)
+  xfocus* 2 (indom (midx \x `[0, Ncol])). (* focus on non-zero getters with `Focus` rule from Fig.5 *)
+  xapp get_spec_out=> //. 1: case=> ??; indomE; tauto.
+  xclean_heap. (* clean up the heap *)
+  have E : (`[0, Nrow] \x `[0, Ncol]) ∩ indom (midx \x `[0, Ncol]) = midx \x `[0, Ncol]. (* simplify index sets *)
+  { rewrite -prod_intr_list_on_1. f_equal. now apply intr_list. }
+  rewrite E (fset_of_list_nodup 0 nodup_midx) len_midx prod_Union_distr.
+  xin 1 : xstep=> s... (* advance the first instruction in `sum` *)
+  xfor_sum Inv R R (fun hv i => Σ_(j <- `{midx[i]} \x `[0, Ncol]) hv[`2](j)) s. (* `For` rule application (Fig.6) *)
+  { xin* 2: xapp* @index.specs; xstep; xwp; xif=> [?|]; xgo...  (* advance all instructions in `ucsr.get` up to `sv.get` *)
+    xin 1 : xgo... (* advance `sum` up to `sv.sum` *)
+    rewrite index_nodup //; try math. (* simplify index *)
+    xsubst (snd : _ -> int). (* apply `Subst` rule from `Fig.7` *)
+    xnapp sv.sum_spec... (*  apply specification for sparse SV vector summation *)
+    xsimpl=>->. xapp @incr.spec. rewrite sum_prod1E. xsimpl. }
+  { move=>Ha Hb Hc; left. move: Ha; apply contrapose, NoDup_nthZ; autos*; math. }
+  xstep. xsimpl*. xsum_normalize. (* adjust summations *)
+  rewrite SumCascade -?prod_Union_distr -?len_midx -?(fset_of_list_nodup 0) ?E //.
+  disjointE.
+  move=>Ha Hb Hc; left. move: Ha; apply contrapose, NoDup_nthZ; autos*; math.
+Qed.
+
+Context (dvec : list int).
+Context (dvec_len : length dvec = Ncol :> int).
+
+(* #9 from the table
+  Dot product of a sparse uCSR matrix and a dense vector *)
+Definition spmv := 
+  <{
+  fun mval midx mind mcrd dvec =>
+  let s = alloc0 Nrow in
+  for i <- [0, Nidx] {
+    let lb = mcrd[i] in
+    let i' = i + 1 in
+    let rb = mcrd[i'] in
+    let i = midx[i ]in
+    let x = sv.dotprod mind mval dvec lb rb in 
+    s[i] := x
+  }; 
+  s
+}>.
+
+(* Specification for `spmv`. Proof is similar to the one above *)
+Lemma spmv_spec `{Inhab D} `{H__ : Inhab (labeled int)} (m_val m_idx m_ind m_crd x_dvec : loc) : 
+  {{ arr(m_val, mval)⟨1, (0,0)⟩ \*
+     arr(m_idx, midx)⟨1, (0,0)⟩ \*
+     arr(m_ind, mind)⟨1, (0,0)⟩ \*
+     arr(m_crd, mcrd)⟨1, (0,0)⟩ \*
+     arr(x_dvec, dvec)⟨1, (0,0)⟩ \* 
+     (\*_(i <- `[0, Nrow] \x `[0, Ncol]) arr(m_val, mval)⟨2, i⟩) \*
+     (\*_(i <- `[0, Nrow] \x `[0, Ncol]) arr(m_idx, midx)⟨2, i⟩) \*
+     (\*_(i <- `[0, Nrow] \x `[0, Ncol]) arr(m_ind, mind)⟨2, i⟩) \*
+     (\*_(i <- `[0, Nrow] \x `[0, Ncol]) arr(m_crd, mcrd)⟨2, i⟩) \*
+     (\*_(i <- `[0, Nrow] \x `[0, Ncol]) arr(x_dvec, dvec)⟨2, i⟩) }}
+  [{
+    [1| _  in `{(0,0)}                 => spmv m_val m_idx m_ind m_crd x_dvec];
+    {2| ij in `[0, Nrow] \x `[0, Ncol] => get m_val m_idx m_ind m_crd ij.1 ij.2}
+  }]
+  {{ hv,
+  arrf(hv[`1]((0, 0)), i0 in Nrow=> Σ_(j0 <- `[0, Ncol]) hv[`2]((i0, j0)) * dvec[j0])⟨1, (0, 0)⟩
+      \* \Top }}.
+Proof with (try seclocal_fold; seclocal_solver).
+  xset_Inv Inv 1; xset_R int Inv R 2.
+  xfocus* 2 (indom (midx \x `[0, Ncol])).
+  xapp get_spec_out=> //. 1: case=> ??; indomE; tauto.
+  xclean_heap.
+  have E : (`[0, Nrow] \x `[0, Ncol]) ∩ indom (midx \x `[0, Ncol]) = midx \x `[0, Ncol].
+  { rewrite -prod_intr_list_on_1. f_equal. now apply intr_list. }
+  rewrite E (fset_of_list_nodup 0 nodup_midx) len_midx prod_Union_distr.
+  xin 1 : xmalloc ans...
+  xfor_arrayset Inv R R 
+    (fun hv (i : int) => (If (In i midx) then Σ_(j <- `{i} \x `[0, Ncol]) (hv[`2](j) * dvec[j.2]) else 0)) 
+    (fun _ : int => 0) ans midx...
+  { xin* 2: xapp* @index.specs; xstep; xwp; xif=> [?|]; xgo...
+    xin 1 : xgo...
+    rewrite index_nodup //; try math.
+    xsubst (snd : _ -> int).
+    xnapp sv.dotprod_spec...
+    xsimpl=>->; xapp; rewrite sum_prod1E; xsimpl.
+    case: classicT=> [?|/(_ (nth_In _ _ _))] //; lia. }
+  xwp; xval. xsimpl*. erewrite -> harray_fun_int_congr; try assumption; first xsimpl*.
+  move=> i Hi /=. xsum_normalize.
+  case_if.
+  { rewrite sum_prod1E /=; apply SumEq=> >; indomE.
+    case: classicT=> // /[swap]? []; exists (index i midx); indomE=> /=.
+    splits; try tauto. 
+    { rewrite -len_midx index_mem //; splits*; exact/(indexG0). }
+    { by rewrite nth_index. } }
+  { rewrite -> SumEq with (G:=fun=> 0)=> [|?]; first by rewrite Sum0s.
+    indomE; case: classicT=> // -[?]; indomE=> /=-[?][*]. 
+    case: C; subst; apply/nth_In; math. }
+Qed.
 
 End unordered_csr.
 
